rocq-osiris/theories/semantics/step.v
@@ -139,47 +139,18 @@ Qed.
 
 (* -------------------------------------------------------------------------- *)
 
-(* [step_store σ l v k] is the right-hand side of the reduction rule [StepStore].
-
-   This rule loads a value [v] from the store [σ] at location [l], overwrites
-   it with the value [v'], and returns a unit value to the continuation [k].
-   It fails if the location [l] is not in the domain of [σ] or contains
-   something other than a value. *)
-
-Definition step_store_1 σ l v' : store :=
-  match σ !! l with
-  | Some (V v) => <[ l := V v' ]> σ
-  | _          => σ
-  end.
-
-Definition step_store_2 {A E} σ l (k : outcome2 val exn → _) : micro A E :=
-  match σ !! l with
-  | Some (V v) => continue k VUnit
-  | _          => crash "store error: unbound location"
-  end.
-
-Notation step_store σ l v' k :=
-  (step_store_1 σ l v', step_store_2 σ l k).
-
-(* Storing is an algebraic effect. *)
-
-Lemma try2_step_store_2 {A B E F} σ l
-  (k : outcome2 val exn → micro A E)
-  (k' : outcome2 A E → micro B F)
-:
-  step_store_2 σ l (pftry2 k k') = try2 (step_store_2 σ l k) k'.
-Proof.
-  unfold step_store_2. intros. case_location_lookup; simplify_eq; eauto.
-Qed.
-
-(* -------------------------------------------------------------------------- *)
-
 (* [step_exchange σ l v k] is the right-hand side of the reduction rule [StepStore].
 
    This rule loads a value [v] from the store [σ] at location [l], overwrites
    it with the value [v'], and returns a unit value to the continuation [k].
    It fails if the location [l] is not in the domain of [σ] or contains
    something other than a value. *)
+
+Definition step_exchange_1 σ l v' : store :=
+  match σ !! l with
+  | Some (V v) => <[ l := V v' ]> σ
+  | _          => σ
+  end.
 
 Definition step_exchange_2 {A E} σ l (k : outcome2 val exn → _) : micro A E :=
   match σ !! l with
@@ -188,7 +159,7 @@ Definition step_exchange_2 {A E} σ l (k : outcome2 val exn → _) : micro A E :
   end.
 
 Notation step_exchange σ l v' k :=
-  (step_store_1 σ l v', step_exchange_2 σ l k).
+  (step_exchange_1 σ l v', step_exchange_2 σ l k).
 
 (* Storing is an algebraic effect. *)
 
@@ -321,7 +292,6 @@ Qed.
 
 Global Hint Resolve
   try2_step_load_2
-  try2_step_store_2
   try2_step_exchange_2
   try2_step_cas_2
   try2_step_resume_2
@@ -395,15 +365,8 @@ Inductive step {A E} : config A E → config A E → Prop :=
         c'
 
   (* If the location [l] exists and contains a value [v], then
-     [stop CStore (l, v')] overwrites this value with [v'];
+     [stop CExchange (l, v')] overwrites this value with [v'];
      otherwise, it crashes. *)
-  | StepStore :
-      ∀ σ l v' k c',
-      c' = step_store σ l v' k →
-      step
-        (σ, Stop CStore (l, v') k)
-        c'
-
   | StepExchange :
       ∀ σ l v' k c',
       c' = step_exchange σ l v' k →
@@ -666,13 +629,13 @@ Proof.
   rewrite Heq. eauto.
 Qed.
 
-Lemma StepStoreSuccess {A E} σ (l : loc) v v' (k : outcome2 val exn → micro A E) :
+Lemma StepExchangeSuccess {A E} σ (l : loc) v v' (k : outcome2 val exn → micro A E) :
   σ !! l = Some (V v) →
   step
-    (σ, Stop CStore (l, v') k)
-    (<[ l := V v' ]> σ, continue k VUnit).
+    (σ, Stop CExchange (l, v') k)
+    (<[ l := V v' ]> σ, continue k v).
 Proof.
-  intros Heq. econstructor. unfold step_store_1, step_store_2.
+  intros Heq. econstructor. unfold step_exchange_1, step_exchange_2.
   rewrite Heq. eauto.
 Qed.
 
@@ -880,16 +843,16 @@ Proof.
 Qed.
 
 (* If the location [l] exists in the store and contains a value,
-   then [stop CStore (l, v')] can step in only one way. *)
+   then [stop CExchange (l, v')] can step in only one way. *)
 
-Lemma invert_step_store {A E} σ l v' v k σ' m' :
+Lemma invert_step_exchange {A E} σ l v' v k σ' m' :
   σ !! l = Some (V v) →
-  @step A E (σ, Stop CStore (l, v') k) (σ', m') →
+  @step A E (σ, Stop CExchange (l, v') k) (σ', m') →
   σ' = <[ l := V v' ]> σ ∧
-  m' = continue k VUnit.
+  m' = continue k v.
 Proof.
   intros Heq Hstep. destruct_step.
-  unfold step_store_1, step_store_2. rewrite Heq.
+  unfold step_exchange_1, step_exchange_2. rewrite Heq.
   eauto.
 Qed.
 
